\documentclass[12pt]{article}

\usepackage{amsmath}
\usepackage{amssymb}

\title{Problem Set 6}
\author{Arjun Ghosh}
\date{\today}

\begin{document}
\maketitle
1. (a)
We know that a wave travelling in the forward direction is given

$$
y_{f} = Ae^{i ( kx - \omega t ) }
$$

(b)
The reflected wave is given
$$
y_{b} = RAe^{i ( kx + \omega t ) }
$$

Thus the complete wave is give
$$
y(x,t) = Ae^{i ( kx + \omega t ) }+ RAe^{i ( kx - \omega t ) }
$$
Setting $y(0,t) = 0$ we have
$$
y(0,t) = A e^{ikx} ( e^{i \omega t} + R e^{-i \omega t} ) \implies R = -1
$$
thus that the reflected wave is the has an amplitude opposiute to the direct wave

(c) 
If the boundary is free then we have
$$\frac{\partial y}{\partial x} = 0
$$
at $x = 0$. Thus we have


\end{document}
